NoC_Modular/FMCAD25/dafny/flit_generation.dfy
@@ -4,7 +4,7 @@ method discrete_uniform(min: int, max: int) returns (val: int)
   requires min <= max 
   ensures {:axiom} min <= val <= max
 
-method generate_flits<T(0)>(this_id: nat, max_id: nat, payload: T) returns (f: Flit)
+method generate_flits(this_id: nat, max_id: nat) returns (f: Flit)
   requires 0 <= this_id <= max_id
   requires 1 <= max_id
   ensures f.destination.Id?
@@ -16,7 +16,7 @@ method generate_flits<T(0)>(this_id: nat, max_id: nat, payload: T) returns (f: F
        then destination + 1 
        else destination;
   
-  f := Flit(Id(dest), payload);
+  f := Flit(Id(dest));
 
   return f;
 }
